rupicola/io/IO.fst
@@ -39,3 +39,41 @@ let rec theta #a (m:io a) : hist a =
   match m with
   | Return x -> hist_return x
   | Call o args k -> hist_bind (op_wp o args) (fun r -> theta (k r))
+
+let post_condition_independence (#a:Type) (#h:history) (p:hist_post h a) (x:a) :
+  Lemma (requires p [] x)
+        (ensures forall h' (p':hist_post h' a). p' [] x) = admit ()
+
+(*let theta_hist_indep #a (m:io a) (h:history) (lt:local_trace h) (fs_r:a) (p:hist_post h a) :
+  Lemma (requires theta m h p ==> p lt fs_r)
+        (ensures forall (h':history). exists (p':hist_post h' a) (lt':local_trace h'). theta m h' p' ==> p' lt' fs_r /\ (lt' == lt) /\ (p == p')) = admit () *)
+
+let theta_history_independence #a (m:io a) (h:history) (lt:local_trace h) (fs_r:a) (p:hist_post h a) :
+  Lemma (requires theta m h p ==> p lt fs_r)
+        (ensures forall h' (lt':local_trace h') p'. theta m h' p' ==> p' lt' fs_r) =
+  introduce forall h' lt' p'. theta m h' p' ==> p' lt' fs_r with begin
+    introduce theta m h' p' ==> p' lt' fs_r with _. begin
+      let _ : hist0 a = theta m in
+      let _ : h:history -> hist_post h a -> Type0 = theta m in
+      let _ : hist_post h a = p in
+      let _ : local_trace h -> a -> Type0 = p in
+      match m with
+      | Return x -> begin
+        assert (theta m h p == (hist_return x) h p);
+        assert (theta m h p == p [] x);
+        assert (p [] x ==> p lt fs_r);
+        assume (p' [] x ==> p' lt' fs_r);
+        ()
+        //admit ()
+        end
+      | Call o args k -> begin
+        //hist_bind (op_wp o args) (fun r -> theta (k r))
+        //fun h p -> (op_wp o args) h (hist_post_bind h (fun r -> theta (k r)) p)
+        assume (theta m h p == (hist_bind (op_wp o args) (fun r -> theta (k r))) h p);
+        assert (theta m h p == (op_wp o args) h (hist_post_bind h (fun r -> theta (k r)) p));
+        assert (theta m h p == (op_wp o args) h (fun lt r -> (fun r -> theta (k r)) r (h++lt) (hist_post_shift h p lt)));
+        assert (theta m h p == (op_wp o args) h (fun lt r -> (fun r -> theta (k r)) r (h++lt) (fun lt' r -> p (lt @ lt') r)));
+        admit ()
+        end
+    end
+  end
